Lemma/Bool/SEq/is/EqCast/of/Eq.lean
@@ -1,6 +1,6 @@
 import stdlib.SEq
 import sympy.Basic
-import sympy.Basic'
+
 
 /--
 | attributes | lemma |
@@ -9,12 +9,11 @@ import sympy.Basic'
 | comm | Bool.EqCast.is.SEq.of.Eq |
 | mp   | Bool.EqCast.of.SEq.Eq |
 | mpr  | Bool.SEq.of.EqCast.Eq |
-| mp.comm 2 | Bool.Eq_Cast.of.SEq.Eq |
-| mpr.comm 1 | Bool.SEq.of.Eq_Cast |
+| mp.comm | Bool.Eq_Cast.of.SEq.Eq |
+| mpr.comm | Bool.SEq.of.Eq_Cast |
 | comm.mp 1 | Bool.SEq.is.Eq_Cast.of.Eq |
 -/
--- @[main, comm, mp, mpr, mp.comm 2, mpr.comm 1]
-@[main, comm.mp' 1]
+@[main, comm, mp, mpr, mp.comm, mpr.comm, comm.is 1]
 private lemma main
   {Vector : α → Sort v}
   {a : Vector n}
@@ -27,21 +26,6 @@ private lemma main
   simp [SEq]
   aesop
 
--- private lemma reverse
---   {Vector : α → Sort v}
---   {a : Vector n}
---   {b : Vector m}
--- -- given
---   (h : n = m) :
--- -- imply
---   b ≃ a ↔ b = cast (by congr) a :=
--- -- proof
---   Iff.intro
---     (Bool.Eq_Cast.of.SEq.Eq h) --mp.comm 2
---     (Bool.SEq.of.Eq_Cast (h := h)) -- mpr.comm 1
--- #check Iff.comm.mp
+
 -- created on 2025-07-25
 -- updated on 2025-10-04
--- #check Bool.Eq_Cast.of.SEq.Eq
--- #check Bool.SEq.of.Eq_Cast
--- #check Iff.intro
