Lemma/Bool/SEq/is/SEqCast/of/Eq.lean
@@ -2,20 +2,20 @@ import stdlib.SEq
 import sympy.Basic
 
 /--
-design tricks : using mpr.comm 1 instead of mpr.comm 2 due to the fact that:
-(h : n_a = n_b')
+design tricks : (h : n_a = n_b')
 proposition `cast (congrArg Vector h) a ≃ b` is dependent on `h`, effectively making h an implicit argument.
-thus the resulted lemma name using attribute mpr.comm 1 is `Bool.SEq.of.SEq_Cast`
+thus the resulted lemma name using attribute mpr.comm is `Bool.SEq.of.SEq_Cast`
 | attributes | lemma |
 | --- | --- |
 | main | Bool.SEq.is.SEqCast.of.Eq |
 | comm | Bool.SEqCast.is.SEq.of.Eq |
 | mp  | Bool.SEqCast.of.SEq.Eq |
 | mpr   | Bool.SEq.of.SEqCast.Eq |
-| mp.comm 2 | Bool.SEq_Cast.of.SEq |
-| mpr.comm 1 | Bool.SEq.of.SEq_Cast |
+| mp.comm | Bool.SEq_Cast.of.SEq |
+| mpr.comm | Bool.SEq.of.SEq_Cast |
+| comm.is 1 | Bool.SEq.is.SEq_Cast.of.Eq |
 -/
-@[main, comm, mp, mpr, mp.comm 2, mpr.comm 1]
+@[main, comm, mp, mpr, mp.comm, mpr.comm, comm.is 1]
 private lemma main
   {Vector : α → Sort v}
   {a : Vector n_a}
