Lemma/Int/Add/ne/Zero/of/Mul/gt/Zero.lean
@@ -1,8 +1,7 @@
-import Lemma.Int.EqSub.of.EqAdd
-import Lemma.Int.NegMul.eq.MulNeg
-import Lemma.Int.MulNeg.eq.NegSquare
-import Lemma.Int.LtNeg_0.of.Gt_0
 import Lemma.Int.GeSquare_0
+import Lemma.Int.LtNeg_0.of.Gt_0
+import Lemma.Int.MulNeg.eq.NegSquare
+import Lemma.INt.EqSub.is.Eq_Add
 import Lemma.Nat.Lt.of.Lt.Le
 open Int Nat
 
